$$-f^n_t=logq^{n+1}_t-logq^n_t\tag{13.1}$$
$$
logq^n_t=logE_tm_{t,t+n}\tag{13.2}
$$
$$
m_{t,t+n}=\prod^n_{j=1}m_{t+j-1,t+j}
$$
$$
\begin{aligned}
logm_{t,t+n}&=\sum^n_{j=1}logm_{t+j-1,t+j}\\
&=nlongm+\alpha(B)\sum^n_{j=1}w_{t+j}
\end{aligned}
$$
exponentiate:
$$
m_{t,t+n}=e^{A+B+C}
$$
where 
$$A=nlogm$$$$B=\sum^n_{j=1}[\frac{\alpha(B)}{B^j}]_+w_t$$
$$
\begin{aligned}
C&=a_0w_{t+n}+(a_0+a_1)w_{t+n-1}+\cdots+(a_0+\cdots+a_{n-1})w_{t+1}\\
&=A_0w_{t+n}+A_1w_{t+n-1}+\cdots+A_{n-1}w_{t+1}\\
&=\sum^{n-1}_{j=0}A_jw_{t+n-j}
\end{aligned}
$$
Take expectation:
$$
E_tm_{t,t+n}=e^{A+B}E_te^C
$$
Logarithmization:
$$
logE_tm_{t,t+n}=nlogm+\sum^n_{j=1}[\frac{\alpha(B)}{B^j}]_+w_t+\sum^{n-1}_{j=0}k(A_j)
$$
代入（13.2）得
$$
logq^n_t=nlogm+\sum^n_{j=1}[\frac{\alpha(B)}{B^j}]_+w_t+\sum^{n-1}_{j=0}k(A_j)
$$
代入（13.1）得
$$
-f^n_t=logm+[\frac{\alpha(B)}{B^{n+1}}]_+w_t+k(A_n)
$$
