由（a）：$$EL_t(m_{t,t+1})=E(logE_tm_{t,t+1}-logm_{t,t+1})\tag{i}$$由$r^1_{t,t+1} = \frac{1}{q^1_t}$，因为$E_tm_{t,t+1}=q^1_t$，所以$E_tm_{t,t+1}=\frac{1}{r^1_{t,t+1}}$，代入（i）得到（ii）
$$
\begin{aligned}
EL_t(m_{t,t+1})&=E(-logr^1_{t,t+1}-logm_{t,t+1})\\
&=-Elogm_{t,t+1}-Elogr^1_{t,t+1}
\end{aligned}
\tag{ii}
$$
对（2）用[[Jensen’s inequality]]，得到$E_tlog(m_{t,t+n}r_{t,t+n}) \leq logE_t(m_{t,t+n}r_{t,t+n})$，由（2），$E_t(m_{t,t+n}r_{t,t+n})=1$，由此得到（6）
$$
E_tlogm_{t,t+n}+E_tlogr_{t,t+n} \leq 0 \tag{6}
$$
由（6），得到$$-E_tlogm_{t,t+n} \geq E_tlogr_{t,t+n} \tag{iii}$$将（iii）代入（ii）得到（5）式